Proof derivate of word nullable iff word in language

Regular.thy
@@ -2,15 +2,34 @@ theory Regular
   imports Words
 begin
 
+(* Regular Languages *) 
+type_synonym 'a RegLang = "'a word set"
+
+primrec pow:: "'a RegLang \<Rightarrow> nat \<Rightarrow> 'a RegLang" 
+  where
+   "pow s 0 = {Epsilon}"|
+   "pow s (Suc n) = {u*v |u v. u:s & v:(pow s n)}"
+
+definition quotient:: "'a RegLang \<Rightarrow> 'a \<Rightarrow> 'a RegLang"
+  where
+  "quotient R a = {w |w. (a . w) \<in> R}"
+
+
+definition concat :: "'a RegLang \<Rightarrow> 'a word set \<Rightarrow> 'a word set" where "concat R S = {u*v |u v. u:R & v:S}"
+
+lemma concat_containment: "a \<in> A \<and> b \<in> B \<Longrightarrow> (a * b) \<in> (concat A B)"
+  apply(auto simp add: concat_def)
+  done
+
+
+lemma concat_epsilon: "Epsilon \<in> (concat A B) \<Longrightarrow> Epsilon \<in> A \<and> Epsilon \<in> B"
+  apply(auto simp add: concat_def epsi_concat)
+  done
+
 
 (* Regulars *)
 datatype 'a regex = None | Const "'a word" | Union "'a regex" "'a regex" | Concat "'a regex" "'a regex"  | Star "'a regex" 
 
-
-primrec pow:: "'a word set \<Rightarrow> nat \<Rightarrow> 'a word set" 
-  where
-   "pow s 0 = {Epsilon}"|
-   "pow s (Suc n) = {u*v |u v. u:s & v:(pow s n)}"
 
 lemma pow_neutral: "Epsilon \<in> pow s 0"
   apply(auto)
@@ -21,7 +40,7 @@ primrec lang:: "'a regex \<Rightarrow> 'a word set"
    "lang None = {}"|
    "lang (Const w) = {w}" |
    "lang (Union r1 r2) = (lang r1) Un (lang r2)" |
-   "lang (Concat r1 r2) = {u*v |u v. u:(lang r1) & v:(lang r2)}"|
+   "lang (Concat r1 r2) = concat (lang r1) (lang r2)"|
    "lang (Star r) = (\<Union>n. pow (lang r) n)"
 
 (* Epsilon is always in the Kleene closure of a regular expression *)
@@ -42,6 +61,53 @@ primrec nullable:: "'a regex \<Rightarrow> bool"
   "nullable (Concat r1 r2) = ((nullable r1) \<and> (nullable r2))" |
   "nullable (Star r) = True"
 
+  
+(* Show a regular expression is nullablle iff epsilon is the language *)
+lemma nullability: "nullable r \<longleftrightarrow> Epsilon \<in> (lang r)"
+  apply(rule)
+  subgoal proof (induct r)
+    case None
+    then show ?case by auto
+  next
+    case (Const x)
+    then show ?case by auto
+  next
+    case (Union r1 r2)
+    then show ?case by auto
+  next
+    case (Concat r1 r2)
+    then have "Epsilon \<in> (lang r1) \<and> Epsilon \<in> (lang r2)" by simp
+    then have "(Epsilon * Epsilon) \<in> (concat (lang r1) (lang r2))" by (simp only: concat_containment)
+    then show ?case by auto
+  next
+    case (Star r)
+    then show ?case by (simp only: epsi_in_star)
+  qed
+  subgoal proof (induct r) (* Epsilon \<in> (lang r) \<longrightarrow> nullable (Star r) *)
+    case None
+    then have "False" by (simp add: lang_def)
+    then show ?case by rule
+  next
+    case (Const x)
+    then show ?case by simp
+  next
+    case IH:(Union r1 r2)
+    then have "Epsilon \<in> (lang r1) \<or> Epsilon \<in> (lang r2)" by simp
+    then have "(nullable r1) \<or> (nullable r2)" by (auto simp only: IH)
+    then show ?case by (auto)
+  next
+    case IH:(Concat r1 r2)
+    then have "Epsilon \<in> lang (Concat r1 r2)" by simp
+    then have "Epsilon \<in> concat (lang r1) (lang r2)" by simp
+    then have "Epsilon \<in> (lang r1) \<and> Epsilon \<in> (lang r2)" by (simp only: concat_epsilon)
+    then show ?case using IH by (simp add: nullable_def IH)
+  next
+    case (Star r)
+    then show ?case by (simp add: nullable_def)
+  qed
+done
+   
+
 
 (* Define derivatives of regular languages *)
 
@@ -59,6 +125,37 @@ primrec deriv_word:: "'a word \<Rightarrow> 'a regex \<Rightarrow> 'a regex"
   where
   "deriv_word Epsilon r = r" |
   "deriv_word (a . u) r = deriv_word u (deriv a r)"
+
+
+lemma derivative_correct: "w \<in> lang (deriv a r) \<longleftrightarrow> (a . w) \<in> lang r"
+  sorry
+
+
+
+theorem "nullable (deriv_word w r) \<Longrightarrow> w \<in> (lang r)"
+proof (induction w arbitrary: r)
+  case Epsilon
+  then have "nullable (deriv_word Epsilon r)" by simp
+  then have "nullable r" by simp
+  then show ?case by (simp add: nullability)
+next
+  case IH:(Con a w)
+  then have "nullable (deriv_word (a . w)  r)" by simp
+  then have "nullable (deriv_word w (deriv a r))" by simp
+  with IH have "w \<in> lang (deriv a r)" by auto
+  then show ?case by (simp add: derivative_correct)
+qed
+  
+theorem "w \<in> (lang r) \<Longrightarrow> nullable (deriv_word w r)"
+proof (induction w arbitrary: r)
+  case Epsilon
+  then show ?case by (simp add: nullability)
+next
+  case IH:(Con a w)
+  then have "w \<in> lang (deriv a r)" by (simp add: derivative_correct)
+  then show ?case using IH by simp
+qed
+
 
 (* Define containment a nullability of derivative *)
 abbreviation contains:: "'a word \<Rightarrow> 'a regex \<Rightarrow> bool"  (infixr "\<in>" 100) where "contains w r \<equiv> nullable (deriv_word w r)" 
